demo cleanup

Dafny/examples/demoChallengeProb1.i.dfy
@@ -64,66 +64,42 @@ define void @rx_message_routine(i8* nocapture readonly %0) local_unnamed_addr #0
   %14 = trunc i32 %13 to i16
   %16 = zext i16 %14 to i32
   %17 = icmp sgt i32 %16, 0
-  br i1 %17, label %18, label %23
-
-18:                                               ; preds = %1
-  store i8 1, i8* @need_to_flash, align 1
-  br label %19
-
-19:                                               ; preds = %18
-  %20 = call i32 (i8*, ...) @printf(i8* getelementptr inbounds ([3 x i8], [3 x i8]* @.str.2, i64 0, i64 0), i8* getelementptr inbounds ([14 x i8], [14 x i8]* @.str.3, i64 0, i64 0))
-  %21 = call i32 (i8*, ...) @printf(i8* getelementptr inbounds ([2 x i8], [2 x i8]* @.str.1, i64 0, i64 0))
-  br label %22
-
-22:                                               ; preds = %19
-  br label %23
-
-23:                                               ; preds = %22, %1
-  %24 = load i8, i8* @brake_state, align 1
-  %25 = trunc i8 %24 to i1
-  %26 = zext i1 %25 to i8
-  store i8 %26, i8* @previous_brake_state, align 1
   ret void
 }
 */
 
-function {:opaque} demo_challenge_prob_1_code(dst:lvm_operand_opr,s:MemState,t:bitWidth,op1:lvm_operand_opr,op2:lvm_operand_opr,
+function {:opaque} demo_challenge_prob_1_code(dst:lvm_operand_opr,s:MemState,op1:lvm_operand_opr,op2:lvm_operand_opr,
                                               var_5:lvm_operand_opr,var_index2:lvm_operand_opr,comp:lvm_operand_opr):lvm_code
 {
     reveal_IntFits();
-    var void := D(Void);
     var index3 := D(Int(3,IntType(8,false)));
     var index2 := D(Int(2,IntType(8,false)));
     var shl_amount := D(Int(8,IntType(1,false)));
 
-    // var var_5:lvm_operand_opr :| var_5 == dst;
     var var_6:lvm_operand_opr :| var_6 == dst;
     var var_7:lvm_operand_opr :| var_7 == dst;
     var var_8:lvm_operand_opr :| var_8 == dst;
-    // var var_9:lvm_operand_opr :| var_9 == dst;
-
-    // var var_index2:lvm_operand_opr :| var_index2 == dst;
 
     lvm_Block(lvm_CCons(Ins(GETELEMENTPTR(var_5,1,op1,index3)),                  // %5 = getelementptr inbounds i8, i8* %0, i64 3
               lvm_CCons(Ins(LOAD(var_6,s,1,var_5)),                              // %6 = load i8, i8* %2, align 1, !tbaa !4
-              lvm_CCons(Ins(ZEXT(var_7,t,var_6,4)),                              // %7 = zext i8 %3 to i32
+              lvm_CCons(Ins(ZEXT(var_7,1,var_6,4)),                              // %7 = zext i8 %3 to i32
               lvm_CCons(Ins(SHL(var_8,var_7,shl_amount)),                        // %8 = shl i32 %7, 8
               lvm_CCons(Ins(GETELEMENTPTR(var_index2,1,op2,index2)),             // %10 = getelementptr inbounds i8, i8* %0, i64 2
               lvm_CCons(Ins(LOAD(var_index2,s,1,var_index2)),                    // %11 = load i8, i8* %10, align 1
-              lvm_CCons(Ins(ZEXT(var_index2,t,var_index2,4)),                    // %12 = zext i8 %11 to i32
+              lvm_CCons(Ins(ZEXT(var_index2,1,var_index2,4)),                    // %12 = zext i8 %11 to i32
               lvm_CCons(Ins(ADD(dst,4,var_8,var_index2)),                        // %13 = add nsw i32 %8, %12
               lvm_CCons(Ins(ICMP(comp,sgt,4,var_8,D(Int(0,IntType(4,false))))),  // %17 = icmp sgt i32 %16, 0 
-              lvm_CCons(Ins(RET(void)),lvm_CNil())))))))))))                     // ret void
+              lvm_CCons(Ins(RET(D(Void))),lvm_CNil())))))))))))                     // ret void
 
 }
 
 lemma lvm_demo_challenge_prob_1(lvm_b0:lvm_codes, lvm_s0:lvm_state, lvm_sN:lvm_state, 
-            dst:lvm_operand_opr,s:MemState,t:bitWidth,op1:lvm_operand_opr,op2:lvm_operand_opr,
+            dst:lvm_operand_opr,op1:lvm_operand_opr,op2:lvm_operand_opr,
             var_5:lvm_operand_opr,var_index2:lvm_operand_opr,comp:lvm_operand_opr)
   returns (lvm_bM:lvm_codes, lvm_sM:lvm_state)
   requires op1.D?;
   requires op2.D?;
-  requires lvm_require(lvm_b0, demo_challenge_prob_1_code(dst,lvm_s0.m,t,op1,op2,var_5,var_index2,comp), lvm_s0, lvm_sN)
+  requires lvm_require(lvm_b0, demo_challenge_prob_1_code(dst,lvm_s0.m,op1,op2,var_5,var_index2,comp), lvm_s0, lvm_sN)
   requires lvm_is_dst_opr(dst, lvm_s0)
   requires lvm_is_src_opr(op1, lvm_s0)
   requires lvm_get_ok(lvm_s0)
@@ -135,7 +111,6 @@ lemma lvm_demo_challenge_prob_1(lvm_b0:lvm_codes, lvm_s0:lvm_state, lvm_sN:lvm_s
   requires ValidOperand(lvm_s0,var_index2);
   requires ValidOperand(lvm_s0,comp);
   requires operandsUnique(lvm_s0,[dst,var_index2,var_5,comp]);
-  // requires dst != var_index2 != var_5 != comp;
 
   requires OperandContents(lvm_s0,op1).Ptr?;
   requires OperandContents(lvm_s0,op2).Ptr?;
@@ -148,8 +123,7 @@ lemma lvm_demo_challenge_prob_1(lvm_b0:lvm_codes, lvm_s0:lvm_state, lvm_sN:lvm_s
 
   ensures ValidOperand(lvm_sM,dst)
   ensures ValidOperand(lvm_sM, var_index2)
-
-  ensures  lvm_get_ok(lvm_sM)
+  ensures lvm_get_ok(lvm_sM)
 
   ensures  !OperandContents(lvm_sM, dst).Void? ==> OperandContents(lvm_sM, dst).Int?;
   ensures  !OperandContents(lvm_sM, dst).Void? ==> OperandContents(lvm_sM, dst).itype.size == 4;
@@ -172,11 +146,11 @@ lemma lvm_demo_challenge_prob_1(lvm_b0:lvm_codes, lvm_s0:lvm_state, lvm_sN:lvm_s
   reveal_ValidData();
   reveal_evalCodeOpaque();
   reveal_eval_code();
-
+  var operands :=[dst,var_index2,var_5,comp];
   var var_7:lvm_operand_opr :| var_7 == dst;
   var var_8:lvm_operand_opr :| var_8 == dst;
 
-  assert demo_challenge_prob_1_code(dst,lvm_s0.m,t,op1,op2,var_5,var_index2,comp).Block?;
+  assert demo_challenge_prob_1_code(dst,lvm_s0.m,op1,op2,var_5,var_index2,comp).Block?;
   assert lvm_b0.hd.Block?;
   assert evalBlock(lvm_b0, lvm_s0, lvm_sN);
 
@@ -184,147 +158,83 @@ lemma lvm_demo_challenge_prob_1(lvm_b0:lvm_codes, lvm_s0:lvm_state, lvm_sN:lvm_s
   lvm_sM := lvm_ltmp1;
   lvm_bM := lvm_ltmp2;
   var lvm_b1:lvm_codes := lvm_get_block(lvm_cM);
-  assert lvm_b1.lvm_CCons?;
-  assert lvm_b1.hd.Ins?;
-  assert lvm_b1.hd.ins.GETELEMENTPTR?;
-  assert lvm_b1.tl.lvm_CCons?;
-  assert lvm_b1.tl.hd.Ins?;
-  assert lvm_b1.tl.hd.ins.LOAD?;
 
-  // var var_5:lvm_operand_opr :| lvm_require(lvm_b1, lvm_code_GetElementPtr(var_5,1,op1,D(Int(2,IntType(8,false)))),lvm_s0, lvm_sM,var_5);
-  // var var_5:lvm_operand_opr :| lvm_require(lvm_b1, lvm_code_GetElementPtr(var_5,1,op1,D(Int(3,IntType(8,false)))),lvm_s0, lvm_sM);
   assert lvm_b1.hd == Ins(GETELEMENTPTR(var_5,1,op1,D(Int(3,IntType(8,false)))));
   assert lvm_sM == lvm_s0;
+
   ghost var lvm_b2, lvm_s2 := lvm_lemma_GetElementPtr(lvm_b1, lvm_s0, lvm_sM, var_5, lvm_s0.m,1,op1,D(Int(3,IntType(8,false))));
-  assert OperandContents(lvm_s2, var_5) 
-        == evalGETELEMENTPTR(lvm_s0.m,1,OperandContents(lvm_s0,op1),Int(3,IntType(8,false)));
   assert lvm_s0.m == lvm_s2.m;
-
-  assert lvm_b2.hd.Ins?;
-  assert lvm_b2.hd.ins.LOAD?;
-
-  assert lvm_s0.m == lvm_s2.m;
-  assert IsValidBid(lvm_s2.m,OperandContents(lvm_s2,var_5).bid);
-  assert IsValidPtr(lvm_s2.m,OperandContents(lvm_s2,var_5).bid,OperandContents(lvm_s2,op1).offset);
-  assert lvm_s2.m == lvm_sM.m;
-
-  // var var_6:lvm_operand_opr :| lvm_require(lvm_b2, lvm_LOAD(var_6,lvm_s2.m,1,var_5), lvm_s2, lvm_sM,var_6);
-    assert ValidOperand(lvm_s2,dst);
+  assert StateNext(lvm_s0,lvm_s2);
 
   ghost var lvm_b3, lvm_s3 := lvm_lemma_Load(lvm_b2, lvm_s2, lvm_sM, dst,1,var_5);
   assert lvm_s3.m == lvm_s2.m;
-  assert !OperandContents(lvm_s3,dst).Ptr?;
+  assert StateNext(lvm_s2,lvm_s3);
+
   if (OperandContents(lvm_s3,dst).Void?) { // LOAD ins failed
     lvm_sM := lvm_s3;
     assert OperandContents(lvm_sM, dst).Void?;
     return;
   }
-    assert OperandContents(lvm_s3,dst).Int? || OperandContents(lvm_s3,dst).Bytes?;
-    assert lvm_b3.hd.Ins?;
-    assert lvm_b3.hd.ins.ZEXT?;
-    assert lvm_b3.hd.ins == ZEXT(var_7,t,dst,4);
-    assert lvm_b3.tl.lvm_CCons?;
-    assert lvm_b3.tl.hd.Ins?;
-    assert lvm_b3.tl.hd.ins.SHL?;
-    assert OperandContents(lvm_s3,dst).Int?; //   requires OperandContents(lvm_s0,op1).Int?;
-   
-    // assert t == OperandContents(lvm_s3,dst).itype.size;// requires t == OperandContents(lvm_s0,op1).itype.size;
-    assert OperandContents(lvm_s3,dst).itype.size < 4;
-  // requires OperandContents(lvm_s0,dst).Int?;
-  // assert OperandContents(lvm_s3,dst).itype.signed;
+  ghost var lvm_b4, lvm_s4 := lvm_lemma_Zext(lvm_b3, lvm_s3, lvm_sM, var_7, 1,dst,4);
+  assert lvm_s3.m == lvm_s4.m;
+  assert StateNext(lvm_s3,lvm_s4);
 
-    ghost var lvm_b4, lvm_s4 := lvm_lemma_Zext(lvm_b3, lvm_s3, lvm_sM, var_7, t,dst,4);
-    assert OperandContents(lvm_s4, var_7).Int?;
-    assert OperandContents(lvm_s4,var_7).val >= 0;
-    assert !OperandContents(lvm_s4,var_7).itype.signed;
-    assert lvm_s3.m == lvm_s4.m;
+  var shl_amount := D(Int(8,IntType(1,false)));
+  ghost var lvm_b5, lvm_s5 := lvm_lemma_Shl(lvm_b4, lvm_s4, lvm_sM, var_8,var_7,shl_amount);
+  assert lvm_s4.m == lvm_s5.m;
+  assert StateNext(lvm_s4,lvm_s5);
 
-    assert lvm_s4.ok;
-    assert !lvm_b4.CNil?;
-    assert lvm_b4.hd.Ins?;
-    assert lvm_b4.hd.ins.SHL?;
-    assert lvm_b4.tl.hd.Ins?;// == lvm_Block(lvm_CCons(Ins(RET(D(Void))),lvm_CNil()));
 
-    // assert lvm_b4.hd
-//    ghost var lvm_b2, lvm_s2 := lvm_lemma_Add(lvm_b1, lvm_s0, lvm_sM, src2, size,src1,val,o);
-    var shl_amount := D(Int(8,IntType(1,false)));
-    assert lvm_s4.ok;
-    var temp :| temp == OperandContents(lvm_s4,var_7).val;
-    ghost var lvm_b5, lvm_s5 := lvm_lemma_Shl(lvm_b4, lvm_s4, lvm_sM, var_8,var_7,shl_amount);
-    assert lvm_s4.m == lvm_s5.m;
+  assert OperandContents(lvm_s5,var_8).itype.size == 4;
+  assert OperandContents(lvm_s5, var_8).val >= 0;
+  assert OperandContents(lvm_s5,var_8).Int?;
 
-    assert OperandContents(lvm_s5,var_8).itype.size == 4;
-    assert OperandContents(lvm_s5, var_8).val >= 0;
-    assert  OperandContents(lvm_s5,var_8).Int?;
+  assert lvm_b5.hd.Ins?;
+  assert lvm_b5.hd.ins.GETELEMENTPTR?;
 
-    var ex:lvm_operand_opr := copyIntOperand(OperandContents(lvm_s5,var_8));
-
-       assert OperandContents(lvm_s5,ex).itype.size == 4;
-    assert OperandContents(lvm_s5, ex).val >= 0;
-    assert  OperandContents(lvm_s5,ex).Int?;
-
-    // assert OperandContents(lvm_s5, var_8).val > temp;
-     assert OperandContents(lvm_s5,ex).itype.size == 4;
-    assert OperandContents(lvm_s5, ex).val >= 0;
-
-    assert lvm_b5.hd.Ins?;
-    assert lvm_b5.hd.ins.GETELEMENTPTR?;
-    assert lvm_s5.ok;
-    assert lvm_b5.lvm_CCons?;
-    assert ValidState(lvm_s5);
-    assert lvm_b5.tl.hd.ins.LOAD?;
-    assert !lvm_b5.tl.tl.CNil?;
-
-    // assert evalCode(lvm_Block(lvm_b5), lvm_s5, lvm_sM,opTest);// lvm_require(lvm_b5, lvm_code_GetElementPtr(var_index2,1,op2,D(Int(2,IntType(8,false)))),lvm_s5, lvm_sM,var_index2);
-    // var var_index2:lvm_operand_opr :| lvm_require(lvm_b5, lvm_code_GetElementPtr(var_index2,1,op2,D(Int(2,IntType(8,false)))),lvm_s5, lvm_sM,var_index2);//evalCode_lax(lvm_Block(lvm_b5), lvm_s5, lvm_sM,var_index2);
-    // assert lvm_b5.hd == Ins(GETELEMENTPTR(var_index2,1,op2,D(Int(2,IntType(8,false)))));
-    assert  OperandContents(lvm_s5,var_8).Int?;
-
-    assert lvm_s4.m.mem == lvm_s5.m.mem;
-    ghost var lvm_b6, lvm_s6 := lvm_lemma_GetElementPtr(lvm_b5, lvm_s5, lvm_sM, var_index2, s,1,op2,D(Int(2,IntType(8,false))));
-    assert lvm_s5.m.mem == lvm_s6.m.mem;
+  ghost var lvm_b6, lvm_s6 := lvm_lemma_GetElementPtr(lvm_b5, lvm_s5, lvm_sM, var_index2, lvm_s5.m,1,op2,D(Int(2,IntType(8,false))));
+  assert lvm_s5.m == lvm_s6.m;
+  assert StateNext(lvm_s5,lvm_s6);
 
     // LOAD now
-    ghost var lvm_b7, lvm_s7 := lvm_lemma_Load(lvm_b6, lvm_s6, lvm_sM, var_index2,1,var_index2);
-    assert lvm_s6.m.mem == lvm_s7.m.mem;
-    if (OperandContents(lvm_s7,var_index2).Void?) { // LOAD ins failed
-      lvm_sM := lvm_s7;
-      assert OperandContents(lvm_sM, var_index2).Void?;
-      return;
-    }
-    assert OperandContents(lvm_s7,var_index2).Int? || OperandContents(lvm_s7,var_index2).Bytes?;
-    
+  ghost var lvm_b7, lvm_s7 := lvm_lemma_Load(lvm_b6, lvm_s6, lvm_sM, var_index2,1,var_index2);
+  assert lvm_s6.m == lvm_s7.m;
+  assert StateNext(lvm_s6,lvm_s7);
+  if (OperandContents(lvm_s7,var_index2).Void?) { // LOAD ins failed
+    lvm_sM := lvm_s7;
+    assert OperandContents(lvm_sM, var_index2).Void?;
+    return;
+  }
+  
+  assert lvm_b7.hd.ins.ZEXT?;
+  ghost var lvm_b8, lvm_s8 := lvm_lemma_Zext(lvm_b7, lvm_s7, lvm_sM, var_index2, 1,var_index2,4);
+  assert StateNext(lvm_s7,lvm_s8);
 
-    assert lvm_b7.hd.ins.ZEXT?;
-    ghost var lvm_b8, lvm_s8 := lvm_lemma_Zext(lvm_b7, lvm_s7, lvm_sM, var_index2, t,var_index2,4);
-    assert OperandContents(lvm_s8,var_index2).itype.size == 4;
+  assert lvm_b8.hd.ins.ADD?;
+  ghost var lvm_b9, lvm_s9 := lvm_lemma_Add(lvm_b8, lvm_s8, lvm_sM, dst,4,dst,var_index2);
+  assert StateNext(lvm_s8,lvm_s9);
 
-    assert lvm_b8.hd.ins.ADD?;
-    ghost var lvm_b9, lvm_s9 := lvm_lemma_Add(lvm_b8, lvm_s8, lvm_sM, dst,4,dst,var_index2);
+  assert operandsUnique(lvm_s9,operands);
+  assert operands[0] == dst && operands[1] == var_index2;
+  assert OperandContents(lvm_s9,var_8).Int?;
 
-    var arr55 :=[dst,var_index2,var_5,comp];
-    assert operandsUnique(lvm_s9,arr55);
-    assert arr55[0] == dst && arr55[1] == var_index2;
-    assert dst != var_index2;
-    assert var_8 != var_index2;
-    assert  OperandContents(lvm_s9,var_8).Int?;
+  ghost var lvm_b10, lvm_s10:= lvm_lemma_Icmp(lvm_b9, lvm_s9, lvm_sM, comp,sgt,4,var_8,D(Int(0,IntType(4,false))));
+  assert StateNext(lvm_s9,lvm_s10);
 
-    ghost var lvm_b10, lvm_s10:= lvm_lemma_Icmp(lvm_b9, lvm_s9, lvm_sM, comp,sgt,4,var_8,D(Int(0,IntType(4,false))));
-    
+  ghost var lvm_b11, lvm_s11:= lvm_lemma_Ret(lvm_b10, lvm_s10, lvm_sM, dst, D(Void));
+  assert StateNext(lvm_s10,lvm_s11);
 
-    ghost var lvm_b11, lvm_s11:= lvm_lemma_Ret(lvm_b10, lvm_s10, lvm_sM, dst, D(Void));
+  assert lvm_b11 == (lvm_CNil());
+  assert eval_code(lvm_Block(lvm_b11), lvm_s10, lvm_sM);
+  lvm_sM := lvm_lemma_empty(lvm_s11,lvm_sM);
+  assert OperandContents(lvm_sM, dst).Int?;
+  assert OperandContents(lvm_sM,dst).itype.size == 4;
+  assert OperandContents(lvm_sM,dst).itype.size >= 4;
 
-    assert lvm_b11 == (lvm_CNil());
-    assert eval_code(lvm_Block(lvm_b11), lvm_s10, lvm_sM);
-    lvm_sM := lvm_lemma_empty(lvm_s11,lvm_sM);
-    assert OperandContents(lvm_sM, dst).Int?;
-    assert OperandContents(lvm_sM,dst).itype.size == 4;
-    // assert OperandContents(lvm_sM,dst).val <= 4;
-
-    assert ValidState(lvm_sM);
-    
-    assert evalCode(lvm_cM, lvm_s0, lvm_sM);
-    reveal_evalCodeOpaque();
+  assert ValidState(lvm_sM);
+  assert StateNext(lvm_s11,lvm_sM);
+  // assert evalCode(lvm_cM, lvm_s0, lvm_sM);
+  // reveal_evalCodeOpaque();
   
 }
 
